theories/Standardisation.v
@@ -1,0 +1,940 @@
+From Coq Require Import CRelationClasses ssrbool.
+From LogRel.AutoSubst Require Import core unscoped Ast Extra.
+From LogRel Require Import Utils BasicAst Computation Notations Context Closed
+  NormalForms NormalEq Weakening UntypedReduction Confluence.
+
+(* Standardisation *)
+
+Reserved Notation "[ t →s u ]" (at level 0, t, u at level 50).
+Reserved Notation "[ t →w u ]" (at level 0, t, u at level 50).
+Reserved Notation "[ t →w* u ]" (at level 0, t, u at level 50).
+
+Inductive red_tag :=
+| RedWh
+| RedWhStar
+| RedStd.
+
+Inductive sred : red_tag -> term -> term -> Set :=
+| sred_rel {w n} : [w →w* tRel n] -> [w →s tRel n]
+| sred_sort {w s} : [w →w* tSort s] -> [w →s tSort s]
+| sred_prod {w A A' B B'} : [w →w* tProd A B] -> [A →s A'] -> [B →s B'] -> [w →s tProd A' B']
+| sred_lambda {w A A' t t'} : [w →w* tLambda A t] -> [t →s t'] -> [w →s tLambda A' t']
+| sred_app {w t t' u u'} : [w →w* tApp t u] -> [t →s t'] -> [u →s u'] -> [w →s tApp t' u']
+| sred_nat {w} : [w →w* tNat] -> [w →s tNat]
+| sred_zero {w} : [w →w* tZero] -> [w →s tZero]
+| sred_succ {w t t'} : [w →w* tSucc t] -> [t →s t'] -> [w →s tSucc t']
+| sred_natelim {w P P' hz hz' hs hs' t t'} :
+  [w →w* tNatElim P hz hs t] ->
+  [P →s P'] -> [hz →s hz'] -> [hs →s hs'] -> [t →s t'] -> [w →s tNatElim P' hz' hs' t']
+| sred_empty {w} : [w →w* tEmpty] -> [w →s tEmpty]
+| sred_emptyelim {w P P' t t'} : [w →w* tEmptyElim P t] -> [P →s P'] -> [t →s t'] -> [w →s tEmptyElim P' t']
+| sred_sig {w A A' B B'} : [w →w* tSig A B] -> [A →s A'] -> [B →s B'] -> [w →s tSig A' B']
+| sred_pair {w A A' B B' a a' b b'} : [w →w* tPair A B a b] -> [a →s a'] -> [b →s b'] ->
+  [w →s tPair A' B' a' b']
+| sred_fst {w t t'} : [w →w* tFst t] -> [t →s t'] -> [w →s tFst t']
+| sred_snd {w t t'} : [w →w* tSnd t] -> [t →s t'] -> [w →s tSnd t']
+| sred_id {w A A' t t' u u'} : [w →w* tId A t u] -> [A →s A'] -> [t →s t'] -> [u →s u'] -> [w →s tId A' t' u']
+| sred_idrefl {w A A' t t'} : [w →w* tRefl A t] -> [A →s A'] -> [t →s t'] -> [w →s tRefl A' t']
+| sred_idelim {w A A' x x' P P' hr hr' y y' e e'} : [w →w* tIdElim A x P hr y e] ->
+  [A →s A'] -> [x →s x'] -> [P →s P'] -> [hr →s hr'] -> [y →s y'] -> [e →s e'] ->
+  [w →s tIdElim A' x' P' hr' y' e']
+| sred_quote {w t t'} : [w →w* tQuote t] -> [t →s t'] -> [w →s tQuote t']
+| sred_step {w t t' u u'} : [w →w* tStep t u] -> [t →s t'] -> [u →s u'] -> [w →s tStep t' u']
+| sred_reflect {w t t' u u'} : [w →w* tReflect t u] -> [t →s t'] -> [u →s u'] -> [w →s tReflect t' u']
+
+| wred_BRed {A a t} :
+  [tApp (tLambda A t) a →w t[a..]]
+| wred_appSubst {t u a} :
+  [t →w u] ->
+  [tApp t a →w tApp u a]
+| wred_natElimSubst {P hz hs n n'} :
+  [n →w n'] ->
+  [tNatElim P hz hs n →w tNatElim P hz hs n']
+| wred_natElimZero {P hz hs} :
+  [tNatElim P hz hs tZero →w hz]
+| wred_natElimSucc {P hz hs n} :
+  [tNatElim P hz hs (tSucc n) →w tApp (tApp hs n) (tNatElim P hz hs n)]
+| wred_emptyElimSubst {P e e'} :
+  [e →w e'] ->
+  [tEmptyElim P e →w tEmptyElim P e']
+| wred_fstSubst {p p'} :
+  [p →w p'] ->
+  [tFst p →w tFst p']
+| wred_fstPair {A B a b} :
+  [tFst (tPair A B a b) →w a]
+| wred_sndSubst {p p'} :
+  [p →w p'] ->
+  [tSnd p →w tSnd p']
+| wred_sndPair {A B a b} :
+  [tSnd (tPair A B a b) →w b]
+| wred_idElimRefl {A x P hr y A' z} :
+  [tIdElim A x P hr y (tRefl A' z) →w hr]
+| wred_idElimSubst {A x P hr y e e'} :
+  [e →w e'] ->
+  [tIdElim A x P hr y e →w tIdElim A x P hr y e']
+| wred_termEvalAlg {t t'} :
+  [t →s t'] ->
+  dnf t' ->
+  closed0 t' ->
+  [tQuote t →w qNat (model.(quote) (erase t'))]
+| wred_termStepAlg {t t' u u' n k k'} :
+  [t →s t'] ->
+  [u →s qNat u'] ->
+  dnf t' ->
+  closed0 t' ->
+  murec (fun k => eval true (tApp (erase t') (qNat u')) k) k = Some (k', qNat n) ->
+  [tStep t u →w qNat k']
+| wred_termReflectAlg {t t' u u' n k k'} :
+  [t →s t'] ->
+  [u →s qNat u'] ->
+  dnf t' ->
+  closed0 t' ->
+  murec (fun k => eval true (tApp (erase t') (qNat u')) k) k = Some (k', qNat n) ->
+  [tReflect t u →w qEvalTm k' n]
+
+| wred_refl {t} : [t →w* t]
+| wred_trans {t u r} :
+  [t →w u] -> [u →w* r] -> [t →w* r]
+
+where "[ t →s u ]" := (sred RedStd t u)
+and "[ t →w u ]" := (sred RedWh t u)
+and "[ t →w* u ]" := (sred RedWhStar t u)
+.
+
+#[local] Lemma redalg_refl : forall t, [t ⤳* t].
+Proof.
+reflexivity.
+Qed.
+
+Lemma sred_refl : forall t, [t →s t].
+Proof.
+induction t; eauto using sred.
+Qed.
+
+Lemma wsred_step : forall t u, [t →w u] -> [t →w* u].
+Proof.
+intros; eauto using sred.
+Qed.
+
+Lemma wsred_trans : forall t u r, [t →w* u] -> [u →w* r] -> [t →w* r].
+Proof.
+intros t u r Hl Hr.
+remember RedWhStar as tag eqn:Htag in *.
+revert r Hr; induction Hl; try discriminate Htag; eauto using sred.
+Qed.
+
+#[local] Instance PreOrder_wsred : CRelationClasses.PreOrder (sred RedWhStar).
+Proof.
+split.
++ intros ?; apply wred_refl.
++ intros ??? **; now eapply wsred_trans.
+Qed.
+
+Lemma redalg_sred_trans : forall t u r, [t →w* u] -> [u →s r] -> [t →s r].
+Proof.
+intros t u r Hr Hs.
+remember RedStd as tag eqn:Htag in Hs.
+revert t Hr.
+induction Hs; try discriminate Htag.
+all: try now (intros; econstructor; eauto using sred, wsred_trans).
+Qed.
+
+Lemma sred_ren : forall tag t t' ρ, sred tag t t' -> sred tag t⟨ρ⟩ t'⟨ρ⟩.
+Proof.
+intros tag t t' ρ Hr; revert ρ; induction Hr; intros ρ; cbn in *; eauto using sred.
++ replace t[a..]⟨ρ⟩ with t⟨upRen_term_term ρ⟩[a⟨ρ⟩..] by now bsimpl.
+  constructor.
++ rewrite quote_ren; [|tea].
+  constructor; eauto using dnf_ren, closed0_ren.
++ rewrite !qNat_ren.
+  erewrite <- (erase_is_closed0_ren_id _ ρ) in e; tea.
+  econstructor; [..|tea]; eauto using dnf_ren, closed0_ren.
+  now rewrite <- (qNat_ren _ ρ).
++ rewrite qEvalTm_ren.
+  erewrite <- (erase_is_closed0_ren_id _ ρ) in e; tea.
+  econstructor; [..|tea]; eauto using dnf_ren, closed0_ren.
+  now rewrite <- (qNat_ren _ ρ).
+Qed.
+
+Lemma sred_subst_gen : forall tag t t', sred tag t t' ->
+  match tag with
+  | RedWh => forall σ, [t[σ] →w t'[σ]]
+  | RedWhStar => forall σ, [t[σ] →w* t'[σ]]
+  | RedStd => forall σ σ' (Hσ : forall n, [σ n →s σ' n]), [t[σ] →s t'[σ']]
+  end.
+Proof.
+assert (Hup : forall σ σ',
+  (forall n : nat, [σ n →s σ' n]) -> forall n : nat, [up_term_term σ n →s up_term_term σ' n]).
+{ intros σ σ' Hσ []; [apply sred_refl|].
+  cbn; unfold funcomp; now apply sred_ren. }
+induction 1; cbn in *; intros.
+all: try eauto 10 using sred, wsred_step.
++ eapply redalg_sred_trans; [|apply Hσ]; eauto.
++ replace t[a..][σ] with t[up_term_term σ][a[σ]..] by now bsimpl.
+  constructor.
++ rewrite quote_subst; [|tea].
+  constructor; eauto using closed0_subst, dnf_closed0_subst, sred_refl.
++ rewrite !qNat_subst.
+  erewrite <- (erase_is_closed0_subst_id _ ) in e; tea.
+  econstructor; [..|tea]; eauto using closed0_subst, dnf_closed0_subst, sred_refl.
+  rewrite <- (qNat_subst _ σ); eauto using sred_refl.
++ rewrite qEvalTm_subst.
+  erewrite <- (erase_is_closed0_subst_id _ ) in e; tea.
+  econstructor; [..|tea]; eauto using closed0_subst, dnf_closed0_subst, sred_refl.
+  rewrite <- (qNat_subst _ σ); eauto using sred_refl.
+Qed.
+
+Lemma sred_subst : forall t t' σ σ', [t →s t'] -> (forall n, [σ n →s σ' n]) ->
+  [t[σ] →s t'[σ']].
+Proof.
+intros; now apply (sred_subst_gen RedStd).
+Qed.
+
+Lemma sred_subst1 : forall t t' u u', [t →s t'] -> [u →s u'] -> [t[u..] →s t'[u'..]].
+Proof.
+intros; apply sred_subst; tea.
+intros []; [tea|apply sred_refl].
+Qed.
+
+Lemma wsred_app : forall t t' u, [t →w* t'] -> [tApp t u →w* tApp t' u].
+Proof.
+intros * Hr.
+remember RedWhStar as tag eqn:Htag in *.
+induction Hr; try discriminate Htag.
++ reflexivity.
++ econstructor; [|eauto].
+  now constructor.
+Qed.
+
+Lemma wsred_natElim : forall P hs hz t t', [t →w* t'] -> [tNatElim P hs hz t →w* tNatElim P hs hz t'].
+Proof.
+intros * Hr.
+remember RedWhStar as tag eqn:Htag in *.
+induction Hr; try discriminate Htag.
++ reflexivity.
++ econstructor; [|eauto].
+  now constructor.
+Qed.
+
+Lemma wsred_fst : forall t t', [t →w* t'] -> [tFst t →w* tFst t'].
+Proof.
+intros * Hr.
+remember RedWhStar as tag eqn:Htag in *.
+induction Hr; try discriminate Htag.
++ reflexivity.
++ econstructor; [|eauto].
+  now constructor.
+Qed.
+
+Lemma wsred_snd : forall t t', [t →w* t'] -> [tSnd t →w* tSnd t'].
+Proof.
+intros * Hr.
+remember RedWhStar as tag eqn:Htag in *.
+induction Hr; try discriminate Htag.
++ reflexivity.
++ econstructor; [|eauto].
+  now constructor.
+Qed.
+
+Lemma wsred_idElim : forall A x P hr y t t', [t →w* t'] -> [tIdElim A x P hr y t →w* tIdElim A x P hr y t'].
+Proof.
+intros * Hr.
+remember RedWhStar as tag eqn:Htag in *.
+induction Hr; try discriminate Htag.
++ reflexivity.
++ econstructor; [|eauto].
+  now constructor.
+Qed.
+
+#[local] Ltac inv_nf := repeat match goal with
+| H : dnf _ |- _ => (inversion H; subst; try match goal with H : dne _ |- _ => now inversion H end); []; clear H
+| H : dne _ |- _ => inversion H; subst; []; clear H
+| H : whnf _ |- _ => (inversion H; subst; try match goal with H : whne _ |- _ => now inversion H end); []; clear H
+| H : whne _ |- _ => inversion H; subst; []; clear H
+end.
+
+Lemma wred_tLambda_inv {A A' t t'} : [tLambda A t →w* tLambda A' t'] -> t = t'.
+Proof.
+remember RedWhStar as tag eqn:Htag.
+remember (tLambda A t) as l eqn:Hl.
+remember (tLambda A' t') as r eqn:Hr.
+intros Hred; revert A A' t t' Hl Hr.
+induction Hred; try discriminate Htag; intros; subst.
++ injection Hr; intros; subst; reflexivity.
++ inversion Hred1.
+Qed.
+
+Lemma sred_tLambda_inv {A A' t t'} : [tLambda A t →s tLambda A' t'] -> [t →s t'].
+Proof.
+inversion 1; subst.
+apply wred_tLambda_inv in H2; now subst.
+Qed.
+
+Lemma wred_tSucc_inv {t t'} : [tSucc t →w* tSucc t'] -> t = t'.
+Proof.
+remember RedWhStar as tag eqn:Htag.
+remember (tSucc t) as l eqn:Hl.
+remember (tSucc t') as r eqn:Hr.
+intros Hred; revert t t' Hl Hr.
+induction Hred; try discriminate Htag; intros; subst.
++ injection Hr; intros; subst; reflexivity.
++ inversion Hred1.
+Qed.
+
+Lemma sred_tSucc_inv {t t'} : [tSucc t →s tSucc t'] -> [t →s t'].
+Proof.
+inversion 1; subst.
+apply wred_tSucc_inv in H1; now subst.
+Qed.
+
+Lemma wred_tPair_inv_fst {A A' B B' a a' b b'} : [tPair A B a b →w* tPair A' B' a' b'] -> a = a'.
+Proof.
+remember RedWhStar as tag eqn:Htag.
+remember (tPair A B a b) as l eqn:Hl.
+remember (tPair A' B' a' b') as r eqn:Hr.
+intros Hred; revert A A' B B' a a' b b' Hl Hr.
+induction Hred; try discriminate Htag; intros; subst.
++ injection Hr; intros; subst; reflexivity.
++ inversion Hred1.
+Qed.
+
+Lemma sred_tPair_inv_fst {A A' B B' a a' b b'} : [tPair A B a b →s tPair A' B' a' b'] -> [a →s a'].
+Proof.
+inversion 1; subst.
+apply wred_tPair_inv_fst in H5; now subst.
+Qed.
+
+Lemma wred_tPair_inv_snd {A A' B B' a a' b b'} : [tPair A B a b →w* tPair A' B' a' b'] -> b = b'.
+Proof.
+remember RedWhStar as tag eqn:Htag.
+remember (tPair A B a b) as l eqn:Hl.
+remember (tPair A' B' a' b') as r eqn:Hr.
+intros Hred; revert A A' B B' a a' b b' Hl Hr.
+induction Hred; try discriminate Htag; intros; subst.
++ injection Hr; intros; subst; reflexivity.
++ inversion Hred1.
+Qed.
+
+Lemma sred_tPair_inv_snd {A A' B B' a a' b b'} : [tPair A B a b →s tPair A' B' a' b'] -> [b →s b'].
+Proof.
+inversion 1; subst.
+apply wred_tPair_inv_snd in H5; now subst.
+Qed.
+
+Lemma sred_pred_trans : forall t u u', [t →s u] -> [u ⇉ u'] -> [t →s u'].
+Proof.
+intros t u; revert t; induction u; intros t u' Hst Hred.
+all: try now inversion Hred.
+all: try now (inversion Hst; subst; inversion Hred; subst; eauto using sred).
++ inversion Hst; subst.
+  inversion Hred; subst.
+  - econstructor; eauto.
+  - inversion H2; subst.
+    eapply redalg_sred_trans; [tea|].
+    eapply redalg_sred_trans; [now eapply wsred_app|].
+    eapply redalg_sred_trans; [apply wsred_step, wred_BRed|].
+    apply sred_subst1; eauto.
+    eapply sred_tLambda_inv, IHu1; eauto using sred, pred.
++ inversion Hst; subst.
+  inversion Hred; subst.
+  - econstructor; eauto.
+  - inversion H8; subst.
+    eapply redalg_sred_trans; [tea|].
+    eapply redalg_sred_trans; [now eapply wsred_natElim|].
+    eapply redalg_sred_trans; [|apply IHu2; tea].
+    apply wsred_step; eauto using sred.
+  - inversion H8; subst.
+    eapply redalg_sred_trans; [tea|].
+    eapply redalg_sred_trans; [now eapply wsred_natElim|].
+    eapply redalg_sred_trans; [apply wsred_step; eauto using sred|].
+    assert [t2 →s t'].
+    { apply sred_tSucc_inv, IHu4; eauto using sred, sred_refl, pred. }
+    econstructor; [reflexivity|..]; [econstructor; [reflexivity|..]|]; eauto using sred.
++ inversion Hst; subst.
+  inversion Hred; subst.
+  - econstructor; eauto.
+  - inversion H1; subst.
+    eapply redalg_sred_trans; [tea|].
+    eapply redalg_sred_trans; [now eapply wsred_fst|].
+    eapply redalg_sred_trans; [apply wsred_step; eauto using sred|].
+    eapply sred_tPair_inv_fst, IHu; [|eauto using pred, pred_refl].
+    econstructor; [reflexivity|..]; eauto.
++ inversion Hst; subst.
+  inversion Hred; subst.
+  - econstructor; eauto.
+  - inversion H1; subst.
+    eapply redalg_sred_trans; [tea|].
+    eapply redalg_sred_trans; [now eapply wsred_snd|].
+    eapply redalg_sred_trans; [apply wsred_step; eauto using sred|].
+    eapply sred_tPair_inv_snd, IHu; [|eauto using pred, pred_refl].
+    econstructor; [reflexivity|..]; eauto.
++ inversion Hst; subst.
+  inversion Hred; subst.
+  - econstructor; eauto.
+  - inversion H12; subst.
+    eapply redalg_sred_trans; [tea|].
+    eapply redalg_sred_trans; [now eapply wsred_idElim|].
+    eapply redalg_sred_trans; [apply wsred_step; eauto using sred|]; eauto.
++ inversion Hst; subst.
+  inversion Hred; subst.
+  - econstructor; eauto.
+  - eapply redalg_sred_trans; [tea|].
+    eapply redalg_sred_trans; [eapply wsred_step, wred_termEvalAlg; eauto|apply sred_refl].
+    now apply dnf_unannot_rev.
++ inversion Hst; subst.
+  inversion Hred; subst.
+  - econstructor; eauto.
+  - eapply redalg_sred_trans; [tea|].
+    eapply redalg_sred_trans; [eapply wsred_step, wred_termStepAlg; eauto|apply sred_refl].
+    now apply dnf_unannot_rev.
++ inversion Hst; subst.
+  inversion Hred; subst.
+  - econstructor; eauto.
+  - eapply redalg_sred_trans; [tea|].
+    eapply redalg_sred_trans; [eapply wsred_step, wred_termReflectAlg; eauto|apply sred_refl].
+Unshelve. all: exact U.
+Qed.
+
+Lemma pred_sred : forall t u, [t ⇉* u] -> [t →s u].
+Proof.
+intros.
+enough (Hg : forall r, [r →s t] -> [r →s u]).
++ apply Hg, sred_refl.
++ induction H; eauto using sred_pred_trans.
+Qed.
+
+#[local] Ltac expandopt :=
+  match goal with H : (bindopt ?x ?f) = Some ?y |- _ =>
+    let Hrw := fresh "Hrw" in
+    destruct (let_opt_some x y f H) as [? Hrw];
+    rewrite Hrw in *; cbn [bindopt] in H
+  end.
+
+#[local] Ltac caseconstr f t :=
+  let b := fresh "b" in
+  let Hb := fresh "Hb" in
+  remember (f t) as b eqn:Hb; destruct b;
+  [destruct t; try discriminate Hb|idtac].
+
+#[local] Ltac caseval := match goal with
+| H : context [if isLambda ?t then _ else _] |- _ =>
+  caseconstr isLambda t
+| H : context [if isNatConstructor ?t then _ else _] |- _ =>
+  caseconstr isNatConstructor t
+| H : context [if isIdConstructor ?t then _ else _] |- _ =>
+  caseconstr isIdConstructor t
+| H : context [if isPairConstructor ?t then _ else _] |- _ =>
+  caseconstr isPairConstructor t
+end.
+
+#[local] Ltac casenf :=
+match goal with
+| H : context [is_whne ?t] |- _ =>
+  let b := fresh "b" in
+  let Hb := fresh "Hb" in
+  remember (is_whne t) as b eqn:Hb; symmetry in Hb; destruct b; [apply is_whne_whne in Hb|]
+| H : context [is_dnf ?t] |- _ =>
+  let b := fresh "b" in
+  let Hb := fresh "Hb" in
+  remember (is_dnf t) as b eqn:Hb; symmetry in Hb; destruct b; [apply is_dnf_dnf in Hb|]
+| H : context [is_closedn 0 ?t] |- _ =>
+  let b := fresh "b" in
+  let Hb := fresh "Hb" in
+  remember (is_closedn 0 t) as b eqn:Hb; symmetry in Hb; destruct b; [|apply UntypedReduction.is_false_not in Hb]
+end.
+
+Lemma dredalg_whne_inv : forall t n, [t ⇶* n] -> dne n -> ∑ t₀, [t ⤳* t₀] × whne t₀ × [t₀ ⇶* n].
+Proof.
+assert (Hnat : forall n, dne (qNat n) -> False).
+{ intros []; inversion 1. }
+assert (Hevaltm : forall n k, dne (qEvalTm n k) -> False).
+{ intros [] ?; inversion 1. }
+intros t n Hr Hn.
+apply dredalg_eval in Hr; [|eauto using dne, dnf].
+destruct Hr as [k Hr].
+revert t n Hr Hn; induction (Wf_nat.lt_wf k) as [k _ IHk]; intros t n Hr Hn.
+destruct t; rewrite UntypedReduction.eval_unfold in Hr.
+all: try injection Hr; intros; subst.
+all: try now inversion Hn.
+all: try (destruct k; [discriminate Hr|]; []).
+all: repeat expandopt; try caseval; try casenf; repeat expandopt.
+all: try discriminate Hr.
+all: try (injection Hr; intros; subst; try now inversion Hn).
++ eexists; split; [|split]; try reflexivity; eauto using whne.
++ apply IHk in Hr; try Lia.lia; eauto.
+  destruct Hr as (r₀&?&?&?); exists r₀; split; [|split]; tea.
+  etransitivity; [|tea].
+  etransitivity; [eapply redalg_app, eval_dredalg; tea|].
+  apply redalg_one_step; constructor.
++ inversion Hn; subst.
+  eexists; split; [|split]; [|now eapply whne_tApp|].
+  - now eapply redalg_app, eval_dredalg.
+  - apply dredalg_app; eauto; now eapply eval_dredalg.
++ apply IHk in Hr; try Lia.lia; eauto.
+  destruct Hr as (r₀&?&?&?); exists r₀; split; [|split]; tea.
+  etransitivity; [|tea].
+  etransitivity; [eapply redalg_natElim, eval_dredalg; tea|].
+  apply redalg_one_step; constructor.
++ apply IHk in Hr; try Lia.lia; eauto.
+  destruct Hr as (r₀&?&?&?); exists r₀; split; [|split]; tea.
+  etransitivity; [|tea].
+  etransitivity; [eapply redalg_natElim, eval_dredalg; tea|].
+  apply redalg_one_step; constructor.
++ inversion Hn; subst.
+  eexists; split; [|split]; [|now eapply whne_tNatElim|].
+  - now eapply redalg_natElim, eval_dredalg.
+  - apply dredalg_natElim; eauto; now eapply eval_dredalg.
++ inversion Hn; subst.
+  eexists; split; [|split]; [|now eapply whne_tEmptyElim|].
+  - now eapply redalg_natEmpty, eval_dredalg.
+  - apply dredalg_emptyElim; eauto; now eapply eval_dredalg.
++ apply IHk in Hr; try Lia.lia; eauto.
+  destruct Hr as (r₀&?&?&?); exists r₀; split; [|split]; tea.
+  etransitivity; [|tea].
+  etransitivity; [eapply redalg_fst, eval_dredalg; tea|].
+  apply redalg_one_step; constructor.
++ inversion Hn; subst.
+  eexists; split; [|split]; [|now eapply whne_tFst|].
+  - now eapply redalg_fst, eval_dredalg.
+  - apply dredalg_fst; eauto; now eapply eval_dredalg.
++ apply IHk in Hr; try Lia.lia; eauto.
+  destruct Hr as (r₀&?&?&?); exists r₀; split; [|split]; tea.
+  etransitivity; [|tea].
+  etransitivity; [eapply redalg_snd, eval_dredalg; tea|].
+  apply redalg_one_step; constructor.
++ inversion Hn; subst.
+  eexists; split; [|split]; [|now eapply whne_tSnd|].
+  - now eapply redalg_snd, eval_dredalg.
+  - apply dredalg_snd; eauto; now eapply eval_dredalg.
++ apply IHk in Hr; try Lia.lia; eauto.
+  destruct Hr as (r₀&?&?&?); exists r₀; split; [|split]; tea.
+  etransitivity; [|tea].
+  etransitivity; [eapply redalg_idElim, eval_dredalg; tea|].
+  apply redalg_one_step; constructor.
++ inversion Hn; subst.
+  eexists; split; [|split]; [|now eapply whne_tIdElim|].
+  - now eapply redalg_idElim, eval_dredalg.
+  - apply dredalg_idElim; eauto; now eapply eval_dredalg.
++ now eelim Hnat.
++ inversion Hn; subst.
+  eexists; split; [|split]; [|now eapply whne_tQuote|].
+  - now eapply redalg_quote, eval_dredalg.
+  - reflexivity.
++ cbn in Hr; casenf; repeat expandopt.
+  - destruct projT3; expandopt; injection Hr; intros; subst; clear Hr.
+    now eelim Hnat.
+  - injection Hr; intros; subst; clear Hr.
+    inversion Hn; subst.
+    eexists; split; [|split]; [..|reflexivity]; eauto using whnf, whne.
+    apply redalg_step; eauto; now eapply eval_dredalg.
++ cbn in Hr; inversion Hn; subst.
+  eexists; split; [|split]; [|now eapply whne_tStep|].
+  - eapply redalg_step; tea; now eapply eval_dredalg.
+  - reflexivity.
++ cbn in Hr; casenf; repeat expandopt.
+  - destruct projT3; expandopt; injection Hr; intros; subst; clear Hr.
+    now eelim Hevaltm.
+  - injection Hr; intros; subst; clear Hr.
+    inversion Hn; subst.
+    eexists; split; [|split]; [..|reflexivity]; eauto using whnf, whne.
+    apply redalg_reflect; eauto; now eapply eval_dredalg.
++ cbn in Hr; casenf; [congruence|].
+  inversion Hn; subst.
+  eexists; split; [|split]; [..|reflexivity]; eauto using whnf, whne.
+  apply redalg_reflect; eauto; now eapply eval_dredalg.
+Qed.
+
+(* Quasi-reduction: reduction up to some annotations *)
+Definition qred deep t u := ∑ u', eqannot u u' × @RedClosureAlg deep t u'.
+
+Lemma qred_dqred : forall t u, qred false t u -> qred true t u.
+Proof.
+intros * [r []]; exists r; split; eauto using gred_red.
+Qed.
+
+Lemma red_qred : forall deep t u, @RedClosureAlg deep t u -> qred deep t u.
+Proof.
+intros; eexists; split; [reflexivity|tea].
+Qed.
+
+Lemma eqannot_red_qred : forall deep t t' u,
+  eqannot t t' -> @OneRedAlg deep t u -> ∑ u', eqannot u u' × @OneRedAlg deep t' u'.
+Proof.
+assert (Hnf : forall t u, unannot t = unannot u -> dnf t -> dnf u).
+{ intros; now eapply dnf_eqannot. }
+assert (Hne : forall t u, unannot t = unannot u -> dne t -> dne u).
+{ intros; now eapply dne_eqannot. }
+assert (Hwhne : forall t u, unannot t = unannot u -> whne t -> whne u).
+{ intros; now eapply whne_eqannot. }
+unfold eqannot; intros deep t t' u Htt' Hr; revert t' Htt'; induction Hr; intros; cbn in *.
+all: try match goal with H : is_true ?deep |- _ => destruct deep; [|discriminate H] end.
+all: repeat match goal with H : _ = unannot ?t |- _ => destruct t; try discriminate H; []; try (injection H; intros; subst); clear H end.
+all: repeat match goal with
+  | H : forall (t' : term), (unannot ?t = unannot t') -> _, H' : unannot ?t = _ |- _ =>
+    specialize (H _ H'); destruct H as (?&?&?)
+  end.
+all: try (eexists; split; [|now constructor; eauto]; []; cbn; congruence).
++ eexists; split; [|constructor].
+  rewrite !unannot_subst1; congruence.
++ eexists; split; [reflexivity|].
+  replace (erase t) with (erase t'); [eauto using @OneRedAlg, closed0_eqannot|].
+  rewrite !erase_unannot_etared; now f_equal.
++ symmetry in H; apply eqannot_qNat_inv in H; subst.
+  eexists; split; [reflexivity|].
+  econstructor; eauto using closed0_eqannot.
+  replace (erase t'1) with (erase t); [eauto using @OneRedAlg, closed0_eqannot|].
+  rewrite !erase_unannot_etared; now f_equal.
++ symmetry in H; apply eqannot_qNat_inv in H; subst.
+  eexists; split; [reflexivity|].
+  econstructor; eauto using closed0_eqannot.
+  replace (erase t'1) with (erase t); [eauto using @OneRedAlg, closed0_eqannot|].
+  rewrite !erase_unannot_etared; now f_equal.
+Qed.
+
+Lemma eqannot_redalg_qred : forall deep t t' u,
+  eqannot t t' -> @RedClosureAlg deep t u -> ∑ u', eqannot u u' × @RedClosureAlg deep t' u'.
+Proof.
+intros deep t t' u Heq Hr; revert t' Heq; induction Hr.
++ intros; eexists; split; [tea|reflexivity].
++ intros t'' Htt''.
+  eapply eqannot_red_qred in o; [|tea].
+  destruct o as (r&?&?).
+  edestruct IHHr as (r'&?&?); [tea|].
+  eexists; split; [tea|]; now econstructor.
+Qed.
+
+Lemma qred_refl : forall deep t, qred deep t t.
+Proof.
+intros; eexists; split; [reflexivity|reflexivity].
+Qed.
+
+Lemma qred_trans : forall deep t u r, qred deep t u -> qred deep u r -> qred deep t r.
+Proof.
+intros * [t' []] [u' [? Hr]].
+eapply eqannot_redalg_qred in Hr; [|tea].
+destruct Hr as (r'&?&?).
+exists r'; split; [|now etransitivity].
+etransitivity; tea.
+Qed.
+
+Lemma sred_dredalg_gen : forall tag t u, sred tag t u ->
+  match tag with
+  | RedWh => forall r, whnf r -> qred false u r -> qred false t r
+  | RedWhStar => forall r, whnf r -> qred false u r -> qred false t r
+  | RedStd => dnf u -> qred true t u
+  end.
+Proof.
+induction 1; try (now constructor); eauto; intros; inv_nf.
+all: try now (eapply qred_dqred, IHsred; eauto using whnf, whne; eapply qred_refl).
++ eapply qred_trans.
+  - apply qred_dqred, IHsred1; [|apply qred_refl]; eauto using whnf, whne.
+  - destruct IHsred2 as (A₀&?&?); tea.
+    destruct IHsred3 as (B₀&?&?); tea.
+    eexists; split; [now apply eqannot_tProd|].
+    eapply dredalg_prod; eauto using dnf_eqannot.
++ eapply qred_trans.
+  - eapply qred_dqred, IHsred1; [|apply qred_refl].
+    eauto using whnf.
+  - destruct IHsred2 as (t''&?&?); [tea|].
+    eexists; split; [|now apply dredalg_lambda].
+    now apply eqannot_tLambda.
++ destruct IHsred2 as (t₀&?&Ht); [eauto using dnf, dne|].
+  apply dredalg_whne_inv in Ht; [|eapply dne_eqannot; tea].
+  destruct Ht as (tn&?&?&?).
+  assert (qred false (tApp t u) (tApp tn u)).
+  { eexists; split; [reflexivity|]; now apply redalg_app. }
+  eapply qred_trans; [eapply qred_dqred, IHsred1; tea|]; eauto using whnf, whne.
+  destruct IHsred3 as (u₀&?&?); [tea|].
+  eexists; split; [|eapply dredalg_app; tea]; [now apply eqannot_tApp|].
+  now eapply dne_eqannot.
++ eapply qred_trans.
+  - eapply qred_dqred, IHsred1; [|apply qred_refl].
+    eauto using whnf.
+  - destruct IHsred2 as (t₀&?&?); tea.
+    eexists; split; [now apply eqannot_tSucc|].
+    now apply dredalg_succ.
++ destruct IHsred5 as (t₀&?&Ht); eauto using dne, dnf.
+  apply dredalg_whne_inv in Ht; [|eapply dne_eqannot; tea].
+  destruct Ht as (tn&?&?&?).
+  assert (qred false (tNatElim P hz hs t) (tNatElim P hz hs tn)).
+  { eexists; split; [reflexivity|]; now apply redalg_natElim. }
+  eapply qred_trans; [eapply qred_dqred, IHsred1; tea|]; eauto using whnf, whne.
+  destruct IHsred2 as (P₀&?&?); tea.
+  destruct IHsred3 as (hz₀&?&?); tea.
+  destruct IHsred4 as (hs₀&?&?); tea.
+  eexists; split; [now apply eqannot_tNatElim|].
+  apply dredalg_natElim; eauto using dne_eqannot, dnf_eqannot.
++ destruct IHsred3 as (t₀&?&Ht); eauto using dne, dnf.
+  apply dredalg_whne_inv in Ht; [|eapply dne_eqannot; tea].
+  destruct Ht as (tn&?&?&?).
+  assert (qred false (tEmptyElim P t) (tEmptyElim P tn)).
+  { eexists; split; [reflexivity|]; now apply redalg_natEmpty. }
+  eapply qred_trans; [eapply qred_dqred, IHsred1; tea|]; eauto using whnf, whne.
+  destruct IHsred2 as (P₀&?&?); tea.
+  eexists; split; [now apply eqannot_tEmptyElim|].
+  apply dredalg_emptyElim; eauto using dne_eqannot, dnf_eqannot.
++ eapply qred_trans.
+  - apply qred_dqred, IHsred1; [|apply qred_refl]; eauto using whnf, whne.
+  - destruct IHsred2 as (A₀&?&?); tea.
+    destruct IHsred3 as (B₀&?&?); tea.
+    eexists; split; [now apply eqannot_tSig|].
+    eapply dredalg_sig; eauto using dnf_eqannot.
++ eapply qred_trans.
+  - apply qred_dqred, IHsred1; [|apply qred_refl]; eauto using whnf, whne.
+  - destruct IHsred2 as (a₀&?&?); tea.
+    destruct IHsred3 as (b₀&?&?); tea.
+    eexists; split; [now apply eqannot_tPair|].
+    now eapply dredalg_pair; eauto using dnf_eqannot.
++ destruct IHsred2 as (t₀&?&Ht); eauto using dnf, dne.
+  apply dredalg_whne_inv in Ht; [|eapply dne_eqannot; tea].
+  destruct Ht as (tn&?&?&?).
+  assert (qred false (tFst t) (tFst tn)).
+  { eexists; split; [reflexivity|]; now apply redalg_fst. }
+  eapply qred_trans; [eapply qred_dqred, IHsred1; tea|]; eauto using whnf, whne.
+  eexists; split; [now apply eqannot_tFst|].
+  now apply dredalg_fst.
++ destruct IHsred2 as (t₀&?&Ht); eauto using dnf, dne.
+  apply dredalg_whne_inv in Ht; [|eapply dne_eqannot; tea].
+  destruct Ht as (tn&?&?&?).
+  assert (qred false (tSnd t) (tSnd tn)).
+  { eexists; split; [reflexivity|]; now apply redalg_snd. }
+  eapply qred_trans; [eapply qred_dqred, IHsred1; tea|]; eauto using whnf, whne.
+  eexists; split; [now apply eqannot_tSnd|].
+  now apply dredalg_snd.
++ eapply qred_trans.
+  - eapply qred_dqred, IHsred1; [|apply qred_refl].
+    eauto using whnf.
+  - destruct IHsred2 as (A₀&?&?); tea.
+    destruct IHsred3 as (t₀&?&?); tea.
+    destruct IHsred4 as (u₀&?&?); tea.
+    eexists; split; [now apply eqannot_tId|].
+    eapply dredalg_id; eauto using dnf_eqannot.
++ eapply qred_trans.
+  - eapply qred_dqred, IHsred1; [|apply qred_refl]; eauto using whnf, whne.
+  - destruct IHsred2 as (A₀&?&?); tea.
+    destruct IHsred3 as (t₀&?&?); tea.
+    eexists; split; [now apply eqannot_tRefl|].
+    eapply dredalg_refl; eauto using dnf_eqannot.
++ destruct IHsred7 as (e₀&?&He); eauto using dnf, dne.
+  apply dredalg_whne_inv in He; [|eapply dne_eqannot; tea].
+  destruct He as (en&?&?&?).
+  assert (qred false (tIdElim A x P hr y e) (tIdElim A x P hr y en)).
+  { eexists; split; [reflexivity|]; now apply redalg_idElim. }
+  eapply qred_trans; [eapply qred_dqred, IHsred1; tea|]; eauto using whnf, whne.
+  destruct IHsred2 as (A₀&?&?); tea.
+  destruct IHsred3 as (x₀&?&?); tea.
+  destruct IHsred4 as (P₀&?&?); tea.
+  destruct IHsred5 as (hr₀&?&?); tea.
+  destruct IHsred6 as (y₀&?&?); tea.
+  eexists; split; [now apply eqannot_tIdElim|].
+  apply dredalg_idElim; eauto using dnf_eqannot, dne_eqannot.
++ eapply qred_dqred, IHsred1; eauto using whnf, whne.
+  destruct IHsred2 as (t₀&?&?); tea.
+  eexists; split; [|now eapply redalg_quote].
+  unfold eqannot; cbn; now f_equal.
++ eapply qred_dqred, IHsred1; eauto using whnf, whne.
+  destruct IHsred2 as (t₀&?&?); tea.
+  destruct IHsred3 as (u₀&?&?); tea.
+  eexists; split; [now apply eqannot_tStep|].
+  apply redalg_step; eauto using dnf_eqannot.
++ eapply qred_dqred, IHsred1; eauto using whnf, whne.
+  destruct IHsred2 as (t₀&?&?); tea.
+  destruct IHsred3 as (u₀&?&?); tea.
+  eexists; split; [now apply eqannot_tReflect|].
+  apply redalg_reflect; eauto using dnf_eqannot.
++ destruct H0 as (r₀&?&?).
+  eexists; split; [tea|].
+  econstructor; [|tea]; constructor.
++ destruct H1 as (r₀&?&Hr).
+  apply redalg_eval in Hr; [|now eapply whnf_eqannot].
+  destruct Hr as [k Hr]; rewrite UntypedReduction.eval_unfold in Hr.
+  destruct k; [discriminate Hr|].
+  expandopt; caseval; try casenf.
+  - apply eval_dredalg in Hrw, Hr.
+    edestruct IHsred as (u₀&Hu₀&?); [|now apply red_qred|]; eauto using whnf, whne.
+    destruct u₀; try discriminate Hu₀; unfold eqannot in Hu₀; cbn in Hu₀; injection Hu₀; intros.
+    eapply eqannot_redalg_qred in Hr; [|eapply eqannot_subst1; tea; reflexivity].
+    destruct Hr as (v&?&?).
+    eexists; split; [etransitivity; tea|].
+    etransitivity; [|tea].
+    etransitivity; [now eapply redalg_app|].
+    do 2 econstructor.
+  - injection Hr; intros; subst; clear Hr; apply eval_dredalg in Hrw.
+    edestruct IHsred as (u₀&Hu₀&?); [|now apply red_qred|]; eauto using whnf, whne.
+    assert (Hred : [tApp t a ⤳* tApp u₀ a]) by now eapply redalg_app.
+    eexists; split; [|tea].
+    etransitivity; [tea|].
+    apply eqannot_tApp; [tea|reflexivity].
+  - discriminate.
++ destruct H1 as (r₀&?&Hr).
+  apply redalg_eval in Hr; [|now eapply whnf_eqannot].
+  destruct Hr as [k Hr]; rewrite UntypedReduction.eval_unfold in Hr.
+  destruct k; [discriminate Hr|].
+  expandopt; caseval; try casenf.
+  - apply eval_dredalg in Hr, Hrw.
+    edestruct IHsred as (n₀&Hn₀&?); [|now apply red_qred|]; eauto using whnf, whne.
+    destruct n₀; try discriminate Hn₀.
+    eexists; split; [tea|].
+    etransitivity; [|tea].
+    etransitivity; [now eapply redalg_natElim|].
+    apply redalg_one_step; constructor.
+  - apply eval_dredalg in Hr, Hrw.
+    edestruct IHsred as (n₀&Hn₀&?); [|now apply red_qred|]; eauto using whnf, whne.
+    destruct n₀; try discriminate Hn₀; unfold eqannot in Hn₀; cbn in Hn₀; injection Hn₀; intros.
+    match type of Hr with [tApp (tApp hs ?r) (tNatElim P hz hs ?r) ⤳* _] =>
+      assert (eqannot (tApp (tApp hs r) (tNatElim P hz hs r)) (tApp (tApp hs n₀) (tNatElim P hz hs n₀)))
+    end.
+    { repeat apply eqannot_tApp; try apply eqannot_tNatElim; tea; reflexivity. }
+    eapply eqannot_redalg_qred in Hr; [|tea].
+    destruct Hr as (r₁&?&?).
+    eexists; split; [etransitivity; tea|].
+    etransitivity; [|tea].
+    etransitivity; [now eapply redalg_natElim|].
+    apply redalg_one_step; constructor.
+  - injection Hr; intros; subst; clear Hr.
+    apply eval_dredalg in Hrw.
+    edestruct IHsred as (n₀&Hn₀&?); [|now apply red_qred|]; eauto using whnf, whne.
+    assert (Hred : [tNatElim P hz hs n ⤳* tNatElim P hz hs n₀]) by now eapply redalg_natElim.
+    eexists; split; [|tea].
+    etransitivity; [tea|]; apply eqannot_tNatElim; tea; reflexivity.
+  - discriminate.
++ eapply qred_trans; [|tea].
+  eexists; split; [reflexivity|].
+  eauto using @OneRedAlg, @RedClosureAlg.
++ destruct H0 as (r₀&?&Hr).
+  eexists; split; [tea|].
+  econstructor; [|tea]; constructor.
++ destruct H1 as (r₀&?&Hr).
+  apply redalg_eval in Hr; [|now eapply whnf_eqannot].
+  destruct Hr as [k Hr]; rewrite UntypedReduction.eval_unfold in Hr.
+  destruct k; [discriminate Hr|].
+  expandopt; try casenf.
+  - injection Hr; intros; subst; clear Hr.
+    apply eval_dredalg in Hrw.
+    edestruct IHsred as (e₀&He₀&?); [|now apply red_qred|]; eauto using whnf, whne.
+    assert (Hred : [tEmptyElim P e ⤳* tEmptyElim P e₀]) by now eapply redalg_natEmpty.
+    eexists; split; [|tea].
+    etransitivity; [tea|]; apply eqannot_tEmptyElim; tea; reflexivity.
+  - discriminate.
++ destruct H1 as (r₀&?&Hr).
+  apply redalg_eval in Hr; [|now eapply whnf_eqannot].
+  destruct Hr as [k Hr]; rewrite UntypedReduction.eval_unfold in Hr.
+  destruct k; [discriminate Hr|].
+  expandopt; caseval; try casenf.
+  - apply eval_dredalg in Hr, Hrw.
+    edestruct IHsred as (p₀&Hp₀&?); [|now apply red_qred|]; eauto using whnf, whne.
+    destruct p₀; try discriminate Hp₀; unfold eqannot in Hp₀; cbn in Hp₀; injection Hp₀; intros.
+    eapply eqannot_redalg_qred in Hr; [|tea].
+    destruct Hr as (r₁&?&?).
+    eexists; split; [etransitivity; tea|].
+    etransitivity; [now eapply redalg_fst|].
+    etransitivity; [|tea].
+    apply redalg_one_step; constructor.
+  - injection Hr; intros; subst; clear Hr.
+    apply eval_dredalg in Hrw.
+    edestruct IHsred as (p₀&Hp₀&?); [|now apply red_qred|]; eauto using whnf, whne.
+    assert (Hred : [tFst p ⤳* tFst p₀]) by now eapply redalg_fst.
+    eexists; split; [|tea].
+    etransitivity; [tea|]; apply eqannot_tFst; tea.
+  - discriminate.
++ destruct H0 as (r₀&?&Hr).
+  eexists; split; [tea|].
+  econstructor; [|tea]; constructor.
++ destruct H1 as (r₀&?&Hr).
+  apply redalg_eval in Hr; [|now eapply whnf_eqannot].
+  destruct Hr as [k Hr]; rewrite UntypedReduction.eval_unfold in Hr.
+  destruct k; [discriminate Hr|].
+  expandopt; caseval; try casenf.
+  - apply eval_dredalg in Hr, Hrw.
+    edestruct IHsred as (p₀&Hp₀&?); [|now apply red_qred|]; eauto using whnf, whne.
+    destruct p₀; try discriminate Hp₀; unfold eqannot in Hp₀; cbn in Hp₀; injection Hp₀; intros.
+    eapply eqannot_redalg_qred in Hr; [|tea].
+    destruct Hr as (r₁&?&?).
+    eexists; split; [etransitivity; tea|].
+    etransitivity; [now eapply redalg_snd|].
+    etransitivity; [|tea].
+    apply redalg_one_step; constructor.
+  - injection Hr; intros; subst; clear Hr.
+    apply eval_dredalg in Hrw.
+    edestruct IHsred as (p₀&Hp₀&?); [|now apply red_qred|]; eauto using whnf, whne.
+    assert (Hred : [tSnd p ⤳* tSnd p₀]) by now eapply redalg_snd.
+    eexists; split; [|tea].
+    etransitivity; [tea|]; apply eqannot_tSnd; tea.
+  - discriminate.
++ destruct H0 as (r₀&?&Hr).
+  eexists; split; [tea|].
+  econstructor; [|tea]; constructor.
++ destruct H0 as (r₀&?&Hr).
+  eexists; split; [tea|].
+  econstructor; [|tea]; constructor.
++ destruct H1 as (r₀&?&Hr).
+  apply redalg_eval in Hr; [|now eapply whnf_eqannot].
+  destruct Hr as [k Hr]; rewrite UntypedReduction.eval_unfold in Hr.
+  destruct k; [discriminate Hr|].
+  expandopt; caseval; try casenf.
+  - apply eval_dredalg in Hr, Hrw.
+    edestruct IHsred as (e₀&He₀&?); [|now apply red_qred|]; eauto using whnf, whne.
+    destruct e₀; try discriminate He₀; unfold eqannot in He₀; cbn in He₀; injection He₀; intros.
+    eexists; split; [tea|].
+    etransitivity; [|tea].
+    etransitivity; [now eapply redalg_idElim|].
+    apply redalg_one_step; constructor.
+  - injection Hr; intros; subst; clear Hr.
+    apply eval_dredalg in Hrw.
+    edestruct IHsred as (e₀&He₀&?); [|now apply red_qred|]; eauto using whnf, whne.
+    assert (Hred : [tIdElim A x P hr y e ⤳* tIdElim A x P hr y e₀]) by now eapply redalg_idElim.
+    eexists; split; [|tea].
+    etransitivity; [tea|]; now apply eqannot_tIdElim.
+  - discriminate.
++ eapply qred_trans with (tQuote t').
+  - destruct IHsred as (t₀&?&?); [tea|].
+    eexists; split; [now apply eqannot_tQuote|].
+    now apply redalg_quote.
+  - destruct H1 as (r₀&?&Hr).
+    eexists; split; [tea|].
+    econstructor; [|tea].
+    now constructor.
++ eapply qred_trans with (tStep t' (qNat u')).
+  - destruct IHsred1 as (t₀&?&?); [tea|].
+    destruct IHsred2 as (u₀&?&?); [apply dnf_qNat|].
+    eexists; split; [apply eqannot_tStep; tea; reflexivity|].
+    eapply redalg_step; eauto using dnf_eqannot, @RedClosureAlg.
+  - destruct H2 as (r₀&?&Hr).
+    eexists; split; [tea|].
+    econstructor; [|tea].
+    now econstructor.
++ eapply qred_trans with (tReflect t' (qNat u')).
+  - destruct IHsred1 as (t₀&?&?); [tea|].
+    destruct IHsred2 as (u₀&?&?); [apply dnf_qNat|].
+    eexists; split; [apply eqannot_tReflect; tea; reflexivity|].
+    eapply redalg_reflect; eauto using dnf_eqannot, @RedClosureAlg.
+  - destruct H2 as (r₀&?&Hr).
+    eexists; split; [tea|].
+    econstructor; [|tea].
+    now econstructor.
+Qed.
+
+Lemma sred_dredalg : forall t u, [t →s u] -> dnf u -> ∑ u', eqannot u u' × [t ⇶* u'].
+Proof.
+intros t u Hr Hnf.
+now eapply (sred_dredalg_gen RedStd).
+Qed.
+
+(* Ad-hoc stuff needed to prove the logical relation *)
+
+Lemma dred_tApp_qNat_compat : forall t t₀ n m,
+  [t ⇶* t₀] -> dnf t₀ ->
+  [tApp t (qNat n) ⇶* qNat m] ->
+  [tApp t₀ (qNat n) ⇶* qNat m].
+Proof.
+intros * Ht Hnf Happ.
+apply dredalg_pred_clos in Ht.
+apply dredalg_pred_clos in Happ.
+eapply pred_clos_app with (u := (qNat n)) in Ht.
+edestruct (pred_confluent) as (v&Hw&Hv); [apply Ht|apply Happ|].
+eapply dnf_pred_clos_id in Hv; [|apply dnf_qNat].
+symmetry in Hv; apply eqannot_qNat_inv in Hv; subst.
+apply pred_sred, sred_dredalg in Hw; [|apply dnf_qNat].
+destruct Hw as (u'&Hu'&?).
+symmetry in Hu'; apply eqannot_qNat_inv in Hu'; now subst.
+Qed.
